First try at changing Hash semantics to be in terms of keys already hashed, not an inverse hash function

src/AsyncDisk.v
@@ -72,9 +72,53 @@ Definition vsmerge (vs : valuset) : list valu := fst vs :: snd vs.
 
 (* Hashing *)
 Definition hashlen := 256.
-
-Parameter hash_inv : word hashlen -> {sz: nat & word sz}.
 Parameter hash_fwd : forall sz, word sz -> word hashlen.
+Definition default_valu : valu := $0.
+Definition default_hash := hash_fwd default_valu.
+
+(* A hashmap holds all keys that Hash has been called on, maps hash values to keys. *)
+Inductive hashmap : Type :=
+  | empty_hashmap : hashmap
+  | upd_hashmap : hashmap -> word hashlen -> { sz : nat & word sz } -> hashmap.
+
+Definition upd_hashmap' hm h sz k : hashmap :=
+  upd_hashmap hm h (existT _ sz k).
+
+Fixpoint hashmap_get hm h : option {sz : nat & word sz} :=
+  if (weq h default_hash)
+    then Some (existT _ _ default_valu) else
+    (match hm with
+    | empty_hashmap => None
+    | upd_hashmap hm' h' k' =>  if (weq h' h)
+                                then Some k'
+                                else hashmap_get hm' h
+    end).
+
+
+Lemma upd_hashmap_eq : forall hm h k,
+  h <> default_hash ->
+  hashmap_get (upd_hashmap hm h k) h = Some k.
+Proof.
+  intros.
+  unfold hashmap_get.
+  destruct (weq h default_hash);
+  destruct (weq h h); intuition.
+Qed.
+
+Lemma upd_hashmap'_eq : forall hm h sz k,
+  h <> default_hash ->
+  hashmap_get (upd_hashmap' hm h k) h = Some (existT _ sz k).
+Proof.
+  intros.
+  unfold upd_hashmap'.
+  apply upd_hashmap_eq; auto.
+Qed.
+
+Hint Rewrite upd_hashmap_eq.
+
+
+Definition hash_safe hm h sz (k : word sz) :=
+  hashmap_get hm h = None \/ hashmap_get hm h = Some (existT _ _ k).
 
 (* Converting between hash and valu.*)
 Lemma hashlen_valulen: hashlen + (valulen - hashlen) = valulen.
